backend/Inlining.v
@@ -374,8 +374,8 @@ Definition expand_instr (ctx: context) (pc: node) (i: instruction): mon unit :=
           set_instr (spc ctx pc) (Inop n)
       end
   | Itailcall sg ros args =>
-      match can_inline ros with
-      | Cannot_inline =>
+      (* match can_inline ros with *)
+      (* | Cannot_inline => *)
           match ctx.(retinfo) with
           | None =>
               set_instr (spc ctx pc)
@@ -384,10 +384,10 @@ Definition expand_instr (ctx: context) (pc: node) (i: instruction): mon unit :=
               set_instr (spc ctx pc)
                         (Icall sg (sros ctx ros) (sregs ctx args) rreg rpc)
           end
-      | Can_inline id f P Q =>
-          do n <- inline_tail_function ctx id f Q args;
-          set_instr (spc ctx pc) (Inop n)
-      end
+      (* | Can_inline id f P Q => *)
+      (*     do n <- inline_tail_function ctx id f Q args; *)
+      (*     set_instr (spc ctx pc) (Inop n) *)
+      (* end *)
   | Ibuiltin ef args res s =>
       set_instr (spc ctx pc)
                 (Ibuiltin ef (map (sbuiltinarg ctx) args) (sbuiltinres ctx res) (spc ctx s))
