common/Memtype.v
@@ -1656,6 +1656,7 @@ for [unchanged_on]. *)
      (INJ: inject j g m1 m2)
      (FAP: frame_at_pos (stack_adt m2) 0 f2)
      (FI: frame_inject' j (perm m1) f1 f2)
+     (SURJ: frameinj_surjective g (length (stack_adt m2)))
      (RSB: record_stack_blocks m1 f1 m1'),
      inject j (fun n : nat => if Nat.eq_dec n 0 then Some O else g (Init.Nat.pred n)) m1' m2;
 
@@ -1669,6 +1670,7 @@ for [unchanged_on]. *)
               forall o k p, perm m2 b o k p -> 0 <= o < frame_size fi) ->
      (forall (b1 b2 : block) (delta : Z), j b1 = Some (b2, delta) -> in_frame fi1 b1 <-> in_frame fi2 b2) ->
      frame_adt_size fi1 = frame_adt_size fi2 ->
+     frameinj_surjective g (length (stack_adt m2)) ->
      record_stack_blocks m1 fi1 m1' ->
      exists m2',
        record_stack_blocks m2 fi2 m2' /\
@@ -1718,6 +1720,7 @@ for [unchanged_on]. *)
    forall (m1 m1' m2 : mem) (j : meminj) g,
      inject j g m1 m2 ->
      unrecord_stack_block m1 = Some m1' ->
+     frameinj_surjective g (length (stack_adt m2)) ->
      g 1%nat = Some O ->
      (forall b, is_stack_top (stack_adt m1) b -> forall o k p, ~ perm m1 b o k p) ->
      inject j (fun n => g (S n)) m1' m2;
@@ -2335,6 +2338,56 @@ Proof.
   eapply IHl in H0. 2: eauto.
   eapply storev_perm_inv; eauto.
 Qed.
+
+Lemma frameinj_surjective_free_list_unrecord:
+  forall g j m P tm tm' tm'' l,
+    free_list tm l = Some tm' ->
+    unrecord_stack_block tm' = Some tm'' ->
+    stack_inject j g P (stack_adt m) (stack_adt tm) ->
+    frameinj_surjective g (length (stack_adt tm)) ->
+    frameinj_surjective (fun n : nat => option_map Init.Nat.pred (g (Datatypes.S n)))
+                        (length (stack_adt tm'')).
+Proof.
+  intros g j m P tm tm' tm'' l FL USB SI SURJ.
+  intros. erewrite <- free_list_stack_blocks in SURJ by eauto.
+  edestruct unrecord_stack_adt as (x & EQ). eauto. rewrite EQ in SURJ.
+  red; intros.
+  destruct (SURJ (S j0)).
+  simpl; omega.
+  destruct (Nat.eq_dec x0 O). subst.
+  {
+    erewrite stack_inject_g0_0 in H0. inv H0. eauto. eapply stack_inject_range in H0; eauto. tauto.
+    eapply stack_inject_range in H0; eauto. omega.
+  }
+  exists (pred x0).
+  replace (S (pred x0)) with x0 by omega. rewrite H0. simpl. auto.  
+Qed.
+
+
+Lemma frameinj_surjective_free_unrecord:
+  forall g j m P tm tm' tm'' b lo hi,
+    free tm b lo hi = Some tm' ->
+    unrecord_stack_block tm' = Some tm'' ->
+    stack_inject j g P (stack_adt m) (stack_adt tm) ->
+    frameinj_surjective g (length (stack_adt tm)) ->
+    frameinj_surjective (fun n : nat => option_map Init.Nat.pred (g (Datatypes.S n)))
+                        (length (stack_adt tm'')).
+Proof.
+  intros g j m P tm tm' tm'' b lo hi FL USB SI SURJ.
+  intros. erewrite <- free_stack_blocks in SURJ by eauto.
+  edestruct unrecord_stack_adt as (x & EQ). eauto. rewrite EQ in SURJ.
+  red; intros.
+  destruct (SURJ (S j0)).
+  simpl; omega.
+  destruct (Nat.eq_dec x0 O). subst.
+  {
+    erewrite stack_inject_g0_0 in H0. inv H0. eauto. eapply stack_inject_range in H0; eauto. tauto.
+    eapply stack_inject_range in H0; eauto. omega.
+  }
+  exists (pred x0).
+  replace (S (pred x0)) with x0 by omega. rewrite H0. simpl. auto.  
+Qed.
+
 
 
 End WITHMEMORYMODEL.
